Kraken/Examples/IndexedSemanticsExample.lean
@@ -1,10 +1,10 @@
 import Kraken.Tactics
 import Kraken.Parser
 import Kraken.Eval
-import Kraken.SimplifiedSemantics
+import Kraken.Variants.IndexedSemantics
 
 open Kraken.Parser
-open Kraken.Simplified
+open Kraken.Indexed
 
 -- This is the same as p2 in Examples, but without using Executable
 def p2 : List Directive := [
@@ -15,27 +15,27 @@ def p2 : List Directive := [
   .instr ⟨ .W64, .W64, .mov Reg.rax (.imm (.int64 2)) ⟩,
 ]
 
--- Replicate the example using the simplified transition relation and polymorphic Eventually
+-- Replicate the example using the indexed transition relation and polymorphic Eventually
 example (s : MachineData) :
-  Eventually (simplified_step1 p2) (fun s' => s'.1.regs.rax = 2) (s, Int64.ofNat 0) := by
+  Eventually (indexed_step1 p2) (fun s' => s'.1.regs.rax = 2) (s, Int64.ofNat 0) := by
   dsimp [p2]
 
   -- initial label
   apply step_cps
-  dsimp only [simplified_step1,Kraken.Simplified.step]
-  simp -- At this point we have simplified the match term from Simplified.step
+  dsimp only [indexed_step1,Kraken.Indexed.step]
+  simp -- At this point we have simplified the match term from step
   dsimp only [Directive.interp, Effects.all]
 
   -- first step: mov
   apply step_cps
-  dsimp only [simplified_step1, Kraken.Simplified.step]
+  dsimp only [indexed_step1, Kraken.Indexed.step]
   simp -- following line does symbolic execution
   dsimp only [Directives.interp,Directive.interp,Instr.interp,Operation.interp,Operand.interp,RegOrMem.interp]
   dsimp only [MachineData.set,Reg64s.set,MachineData.setReg,Reg64s.set64,ConstExpr.interp,CondCode.interp,StatusFlags.from_result, Effects.all]
 
   -- second step: xor %rax, %rax
   apply step_cps
-  dsimp only [simplified_step1, Kraken.Simplified.step]
+  dsimp only [indexed_step1, Kraken.Indexed.step]
   simp
   dsimp only [Directives.interp,Directive.interp,Instr.interp,Operation.interp,Operand.interp,RegOrMem.interp]
   dsimp only [MachineData.set,Reg64s.set,MachineData.setReg,Reg64s.set64,ConstExpr.interp,CondCode.interp,StatusFlags.from_result, Effects.all]
@@ -48,12 +48,12 @@ example (s : MachineData) :
 
   -- third step: jnz
   apply step_cps
-  dsimp only [simplified_step1, Kraken.Simplified.step]
+  dsimp only [indexed_step1, Kraken.Indexed.step]
   simp
 
   -- fifth step: mov
   apply step_cps
-  dsimp only [simplified_step1, Kraken.Simplified.step]
+  dsimp only [indexed_step1, Kraken.Indexed.step]
   simp
   apply Eventually.done
   dsimp [MachineData.setReg, Reg64s.set, Reg64s.set64, ConstExpr.interp]
